Fix compilation warnings
Fixes issue #4

noalias.v
@@ -20,7 +20,6 @@ Require Import heaps.
 Set Implicit Arguments.
 Unset Strict Implicit.
 Import Prenex Implicits.
-Set Automatic Coercions Import.
 
 (******************************************************************************)
 (* noaliasR :                                                                 *)
@@ -41,7 +40,7 @@ Set Automatic Coercions Import.
 
 (* Collect pointers in a heap *)
 Module Scan.
-
+Section ScanSection.
 (* The algorithm is defined as follows:
    - if the heap is h1 :+ h2, then recurse over h1 and h2 and concatenate the
      results.
@@ -50,7 +49,8 @@ Module Scan.
 *)
 
 (* Structure to control the flow of the algorithm *)
-Structure tagged_heap := Tag {untag :> heap}.
+Structure tagged_heap := Tag {untag : heap}.
+Local Coercion untag : tagged_heap >-> heap.
 
 Definition default_tag := Tag.
 Definition ptr_tag := default_tag.
@@ -60,7 +60,8 @@ Definition axiom h s :=
   def h -> uniq s /\ forall x, x \in s -> x \in dom h.
 
 (* Main structure *)
-Structure form s := Form {heap_of :> tagged_heap; _ : axiom heap_of s}.
+Structure form s := Form {heap_of : tagged_heap; _ : axiom heap_of s}.
+Local Coercion heap_of : form >-> tagged_heap.
 
 Lemma union_pf s1 s2 (h1 : form s1) (h2 : form s2) :
         axiom (union_tag (h1 :+ h2)) (s1 ++ s2).
@@ -92,16 +93,20 @@ Proof. by move=>D; split. Qed.
 
 Canonical Structure default_form h := Form (@default_pf h).
 
+Lemma scanE s (h : form s) x : def h -> x \in s -> x \in dom h.
+Proof. by case: h=>hp /= A D H; exact: ((proj2 (A D)) _ H). Qed.
+
+End ScanSection.
+
 (* Pack the exports, as they are not automatically exported by Coq *)
 Module Exports.
 Canonical Structure union_tag.
 Canonical Structure union_form.
 Canonical Structure ptr_form.
 Canonical Structure default_form.
+Coercion untag : tagged_heap >-> heap.
+Coercion heap_of : form >-> tagged_heap.
 End Exports.
-
-Lemma scanE s (h : form s) x : def h -> x \in s -> x \in dom h.
-Proof. by case: h=>hp /= A D H; exact: ((proj2 (A D)) _ H). Qed.
 
 End Scan.
 
@@ -116,14 +121,15 @@ Abort.
 
 (* Search a pointer in a list. Could be generalize to any type *)
 Module Search.
-
+Section SearchSection.
 (* The algorithm is defined as follow:
    - test if the list is (x :: s) for x being the element we are looking for
    - if the list is (y :: s), then recurse using s
 *)
 
 (* Stucture for controlling the flow of the algorithm *)
-Structure tagged_seq := Tag {untag :> seq ptr}.
+Structure tagged_seq := Tag {untag : seq ptr}.
+Local Coercion untag : tagged_seq >-> seq.
 
 Definition recurse_tag := Tag.
 Canonical Structure found_tag s := recurse_tag s.
@@ -131,7 +137,8 @@ Canonical Structure found_tag s := recurse_tag s.
 Definition axiom x (s : tagged_seq) := x \in untag s.
 
 (* Main structure *)
-Structure form x := Form {seq_of :> tagged_seq; _ : axiom x seq_of}.
+Structure form x := Form {seq_of : tagged_seq; _ : axiom x seq_of}.
+Local Coercion seq_of : form >-> tagged_seq.
 
 Lemma found_pf x s : axiom x (found_tag (x :: s)).
 Proof. by rewrite /axiom inE eq_refl. Qed.
@@ -145,14 +152,18 @@ Proof. by move:f=>[[s]]; rewrite /axiom /= inE orbC => ->. Qed.
 Canonical Structure recurse_form x y (f : form x) :=
   Form (recurse_pf y f).
 
+Lemma findE x (f : form x) : x \in untag f.
+Proof. by move:f=>[s]; apply. Qed.
+
+End SearchSection.
+
 Module Exports.
 Canonical Structure found_tag.
 Canonical Structure found_form.
 Canonical Structure recurse_form.
+Coercion untag : tagged_seq >-> seq.
+Coercion seq_of : form >-> tagged_seq.
 End Exports.
-
-Lemma findE x (f : form x) : x \in untag f.
-Proof. by move:f=>[s]; apply. Qed.
 
 End Search.
 
@@ -164,7 +175,7 @@ Abort.
 
 (* Search for two different pointers in a list *)
 Module Search2.
-
+Section Search2Section.
 (* The algorithm works as follow: Let x and y be the pointers we are looking for
    - If we found x, then search for y using the previous module
    - If we found y, then search for x using the previous module
@@ -172,7 +183,8 @@ Module Search2.
 *)
 
 (* Stucture for controlling the flow of the algorithm *)
-Structure tagged_seq := Tag {untag :> seq ptr}.
+Structure tagged_seq := Tag {untag : seq ptr}.
+Local Coercion untag : tagged_seq >-> seq.
 
 Definition foundz_tag := Tag.
 Definition foundy_tag := foundz_tag.
@@ -182,9 +194,8 @@ Definition axiom (x y : ptr) (s : tagged_seq) :=
   [/\ x \in untag s, y \in untag s & uniq s -> x != y].
 
 (* Main structure *)
-Set Record Elimination Schemes.
-Structure form x y := Form {seq_of :> tagged_seq; _ : axiom x y seq_of}.
-Unset Record Elimination Schemes.
+Structure form x y := Form {seq_of : tagged_seq; _ : axiom x y seq_of}.
+Local Coercion seq_of : form >-> tagged_seq.
 
 Lemma foundx_pf x y (s : Search.form y) : axiom x y (foundx_tag (x :: s)).
 Proof.
@@ -214,15 +225,19 @@ Qed.
 Canonical Structure foundz_form x y z (s : form x y) :=
   Form (foundz_pf z s).
 
+Lemma find2E x y (s : form x y) : uniq s -> x != y.
+Proof. by move: s=>[s /= [_ _]]; apply. Qed.
+
+End Search2Section.
+
 Module Exports.
 Canonical Structure foundx_tag.
 Canonical Structure foundx_form.
 Canonical Structure foundy_form.
 Canonical Structure foundz_form.
+Coercion untag : tagged_seq >-> seq.
+Coercion seq_of : form >-> tagged_seq.
 End Exports.
-
-Lemma find2E x y (s : form x y) : uniq s -> x != y.
-Proof. by move: s=>[s /= [_ _]]; apply. Qed.
 
 End Search2.
 
@@ -235,31 +250,37 @@ Abort.
 
 (* Now package everything together *)
 Module NoAlias.
-
+Section NoAliasSection.
 (* The paper describes the reason for this module *)
 
-Structure tagged_ptr (y : ptr) := Tag {untag :> ptr}.
+Structure tagged_ptr (y : ptr) := Tag {untag : ptr}.
+Local Coercion untag : tagged_ptr >-> ptr.
 
 (* Force the unification of y with what appears in the goal *)
 Definition singleton y := @Tag y y.
 
 (* Main structure *)
 Structure form x y (s : seq ptr) :=
-  Form {y_of :> tagged_ptr y;
-         _ : uniq s -> x != untag y_of}.
+  Form {y_of : tagged_ptr y;
+        _ : uniq s -> x != untag y_of}.
+Local Coercion y_of : form >-> tagged_ptr.
 
-Implicit Arguments Form [].
+Arguments Form : clear implicits.
 
 Lemma noalias_pf (x y : ptr) (f : Search2.form x y) :
         uniq f -> x != singleton y.
 Proof. by move: f=>[[s]][]. Qed.
 
 Canonical Structure start x y (f : Search2.form x y) :=
-  @Form x y f (singleton y) (@noalias_pf x y f).
+  Form x y f (singleton y) (@noalias_pf x y f).
+
+End NoAliasSection.
 
 Module Exports.
 Canonical Structure singleton.
 Canonical Structure start.
+Coercion untag : tagged_ptr >-> ptr.
+Coercion y_of : form >-> tagged_ptr.
 End Exports.
 
 End NoAlias.
@@ -270,7 +291,7 @@ Lemma noaliasR s x y (f : Scan.form s) (g : NoAlias.form x y s) :
                def f -> x != NoAlias.y_of g.
 Proof. by move: f g=>[[h]] H1 [[y']] /= H2; case/H1=>U _; apply: H2. Qed.
 
-Implicit Arguments noaliasR [s x y f g].
+Arguments noaliasR [s x y f g].
 Prenex Implicits noaliasR.
 
 Example exnc A (x1 x2 x3 x4 : ptr) (v1 v2 : A) (h1 h2 : heap) :
@@ -324,7 +345,7 @@ case: f D=>[h/=].
 move=>H D; by case: H.
 Qed.
 
-Implicit Arguments noaliasR_fwd1 [s f g].
+Arguments noaliasR_fwd1 [s f] D x y [g].
 
 Notation noaliasR_fwd D x y := (noaliasR_fwd1 D x y (Logic.eq_refl _)).
 Notation "()" := (Logic.eq_refl _).
@@ -354,10 +375,10 @@ Lemma scan_it s (f : Scan.form s) : def f -> uniq s.
 case: f=>/= h A D.
 by case: A.
 Qed.
-Implicit Arguments scan_it [s f].
+Arguments scan_it [s f].
 
 Definition search_them x y g := @Search2.find2E x y g.
-Implicit Arguments search_them [g].
+Arguments search_them x y [g].
 
 Example without_notation
  A (x1 x2 x3 : ptr) (v1 v2 v3 : A) (h1 h2 : heap) :
@@ -422,7 +443,7 @@ case: A g=>// U _ [y' /= ->].
 by apply.
 Qed.
 
-Implicit Arguments noaliasR_fwd3 [s f g].
+Arguments noaliasR_fwd3 [s f] D x y [g].
 
 Example triggered
  A (x1 x2 x3 : ptr) (v1 v2 v3 : A) (h1 h2 : heap) :
