stlogR.v
@@ -15,7 +15,6 @@
     along with this program.  If not, see <http://www.gnu.org/licenses/>.
 *)
 
-Set Automatic Coercions Import.
 
 From mathcomp.ssreflect Require Import ssreflect ssrbool ssrnat eqtype seq ssrfun.
 Require Import heaps rels hprop stmod stsep stlog.
